unitb/decomposition/component.lean
@@ -1,0 +1,77 @@
+
+import unitb.models.nondet
+
+namespace d
+
+open nondet unitb function
+
+section
+
+parameter α : Type
+
+@[reducible]
+private def pred := α → Prop
+
+parameter {α}
+
+structure program : Type 2 :=
+  (asm : α → α → Prop)
+  (mch : nondet.program α)
+
+def compatible {t : Type} (m : t → program) : Prop :=
+∀ i j, i ≠ j → ∀ s s', is_step (m i).mch s s' → (m i).asm s s'
+
+def compose {t : Type} (m : t → program) {s₀ : α}
+  (h₀ : ∀ i, (m i).mch.first s₀)
+  (h : compatible m)
+: program :=
+{ mch :=
+    { lbl := Σ i, (m i).mch.lbl
+    , lbl_is_sched := sorry
+    , first := λ s, ∀ i, (m i).mch.first s
+    , first_fis := ⟨_,h₀⟩
+    , event' := λ i, (m i.1).mch.event' i.2 }
+, asm := sorry }
+
+def step (p : program) (s s' : α) : Prop :=
+nondet.is_step p.mch s s' ∨ p.asm s s'
+
+instance : system program :=
+{ σ := α
+, init := nondet.program.init ∘ program.mch
+, step := step
+, transient := nondet.program.transient ∘ program.mch
+, transient_false := λ s, @system.transient_false _ _ s.mch
+, transient_antimono := λ s, @system.transient_antimono _ _ s.mch }
+
+structure program.ex (s : program) (τ : stream α) : Prop :=
+    (init : s.mch.first (τ 0))
+    (safety : unitb.saf_ex s τ)
+    (liveness : ∀ e, fair' s.mch e τ)
+
+lemma ex_of_ex_mch (s : program) (τ : stream α)
+  (h : s.mch.ex τ)
+: s.ex τ :=
+begin
+  apply d.program.ex.mk,
+  { apply h.init },
+  { unfold saf_ex,
+    apply temporal.henceforth_entails_henceforth _ _ h.safety,
+    apply temporal.action_entails_action,
+    intros s s',
+    unfold unitb.step has_safety.step is_step step,
+    apply or.intro_left },
+  { apply h.liveness },
+end
+
+instance : system_sem program :=
+{ (_ : system program) with
+  ex := λ p, program.ex p
+, init_sem  := λ s p τ Hτ H₀, by { apply H₀, apply Hτ.init }
+, inhabited := λ s, exists_imp_exists (ex_of_ex_mch s) (system_sem.inhabited s.mch)
+, safety    := λ s p, d.program.ex.safety
+, transient_sem := λ s p q τ Hτ T, by apply transient.semantics' _ Hτ.liveness T }
+
+end
+
+end d
