Makefile
@@ -1,5 +1,5 @@
 
-.PHONY: all root logic models refinement syntax clean lines
+.PHONY: all root logic models refinement syntax clean lines decomposition
 
 LEAN_OPT =
 LEAN_PATH = $(shell pwd):/usr/local/bin/../lib/lean/library:$(shell printenv LEAN_PATH)
@@ -7,7 +7,7 @@ LEAN_PATH = $(shell pwd):/usr/local/bin/../lib/lean/library:$(shell printenv LEA
 all:
 	LEAN_PATH=$(LEAN_PATH) lean $(LEAN_OPT) --make > errors.txt
 
-root: logic models refinement syntax util/data/array.olean code
+root: logic models refinement syntax decomposition util/data/array.olean code
 
 logic: unitb/logic/liveness.olean unitb/refinement/basic.olean
 
@@ -19,8 +19,10 @@ refinement: unitb/refinement/resched_data_ref.olean unitb/refinement/split.olean
 
 syntax: unitb/syntax/exists.olean unitb/syntax/simple/machine.olean
 
+decomposition: unitb/decomposition/component.olean
+
 %.olean: %.lean $(shell lean $< --deps)
-	LEAN_PATH=$(LEAN_PATH) lean $(LEAN_OPT) $<
+	LEAN_PATH=$(LEAN_PATH) lean $(LEAN_OPT) --make $<
 
 clean:
 	/usr/bin/find . -name "*.olean" -delete
